Progress

x86/FlatAsm.v
@@ -924,139 +924,140 @@ Definition list_of_segments (p:program) : list segment  :=
   (p.(data_seg) :: (fst p.(code_seg)) :: nil).
 
 Definition undef_seg_block := 1%positive.
-Definition code_block := 2%positive.
-Definition data_block := 3%positive.
+Definition data_block := 2%positive.
+Definition code_block := 3%positive.
+Definition init_block := data_block.
 (* Definition init_glob_block := 4%positive. *)
 
-(* Definition gen_segblocks (p:program) : (segid_type -> block) := *)
-(*   let initmap := fun id => undef_seg_block in *)
-(*   let ids := List.map segid (list_of_segments p) in *)
-(*   acc_segblocks init_block ids initmap. *)
+Definition gen_segblocks (p:program) : (segid_type -> block) :=
+  let initmap := fun id => undef_seg_block in
+  let ids := List.map segid (list_of_segments p) in
+  acc_segblocks init_block ids initmap.
 
-(* Lemma acc_segblocks_upper_bound : forall l i f, *)
-(*   (forall id, Plt (f id) i) -> *)
-(*   (forall id, Plt (acc_segblocks i l f id) (pos_advance_N i (length l))). *)
-(* Proof. *)
-(*   induction l; intros. *)
-(*   - simpl in *. auto. *)
-(*   - simpl in *. destruct ident_eq. *)
-(*     + rewrite psucc_advance_Nsucc_eq. apply Pos.le_lt_trans with (pos_advance_N i (Datatypes.length l)). *)
-(*       apply pos_advance_N_ple. apply Plt_succ. *)
-(*     + apply IHl. intros. apply Plt_trans with i. apply H. *)
-(*       apply Plt_succ. *)
-(* Qed. *)
+Lemma acc_segblocks_upper_bound : forall l i f,
+  (forall id, Plt (f id) i) ->
+  (forall id, Plt (acc_segblocks i l f id) (pos_advance_N i (length l))).
+Proof.
+  induction l; intros.
+  - simpl in *. auto.
+  - simpl in *. destruct ident_eq.
+    + rewrite psucc_advance_Nsucc_eq. apply Pos.le_lt_trans with (pos_advance_N i (Datatypes.length l)).
+      apply pos_advance_N_ple. apply Plt_succ.
+    + apply IHl. intros. apply Plt_trans with i. apply H.
+      apply Plt_succ.
+Qed.
 
-(* Lemma gen_segblocks_upper_bound : forall p id, *)
-(*   Plt (gen_segblocks p id) (pos_advance_N init_block (length (list_of_segments p))). *)
-(* Proof. *)
-(*   intros. unfold gen_segblocks. *)
-(*   eapply acc_segblocks_upper_bound; eauto. *)
-(*   intros. unfold undef_seg_block, init_block. apply Plt_succ. *)
-(* Qed. *)
+Lemma gen_segblocks_upper_bound : forall p id,
+  Plt (gen_segblocks p id) (pos_advance_N init_block (length (list_of_segments p))).
+Proof.
+  intros. unfold gen_segblocks.
+  eapply acc_segblocks_upper_bound; eauto.
+  intros. unfold undef_seg_block, init_block. apply Plt_succ.
+Qed.
 
-(* (* The ids used to create a mapping from segment ids to blocks  *) *)
-(* (*    are indeed mapped to valid blocks by the mapping*) *)
-(* Lemma acc_segblocks_in_valid: forall ids id sbmap initb initmap, *)
-(*   In id ids -> *)
-(*   sbmap = acc_segblocks initb ids initmap -> *)
-(*   segblock_is_valid initb (length ids) (sbmap id). *)
-(* Proof. *)
-(*   clear. *)
-(*   induction ids. intros. *)
-(*   - inv H. *)
-(*   - intros id sbmap initb initmap H H0. simpl in H. destruct H. *)
-(*     subst. simpl. destruct ident_eq. *)
-(*     apply init_segblock_is_valid. omega. congruence. *)
-(*     simpl in H0. subst. destruct ident_eq. *)
-(*     apply init_segblock_is_valid. simpl. omega. *)
-(*     exploit (IHids id (acc_segblocks (Pos.succ initb) ids initmap)); eauto. *)
-(*     intros VALID. unfold segblock_is_valid in *.  destruct VALID. *)
-(*     split. apply Ple_trans with (Pos.succ initb); auto. *)
-(*     apply Ple_succ. simpl. *)
-(*     auto. *)
-(* Qed. *)
+(* The ids used to create a mapping from segment ids to blocks  *)
+(*    are indeed mapped to valid blocks by the mapping*)
+Lemma acc_segblocks_in_valid: forall ids id sbmap initb initmap,
+  In id ids ->
+  sbmap = acc_segblocks initb ids initmap ->
+  segblock_is_valid initb (length ids) (sbmap id).
+Proof.
+  clear.
+  induction ids. intros.
+  - inv H.
+  - intros id sbmap initb initmap H H0. simpl in H. destruct H.
+    subst. simpl. destruct ident_eq.
+    apply init_segblock_is_valid. omega. congruence.
+    simpl in H0. subst. destruct ident_eq.
+    apply init_segblock_is_valid. simpl. omega.
+    exploit (IHids id (acc_segblocks (Pos.succ initb) ids initmap)); eauto.
+    intros VALID. unfold segblock_is_valid in *.  destruct VALID.
+    split. apply Ple_trans with (Pos.succ initb); auto.
+    apply Ple_succ. simpl.
+    auto.
+Qed.
     
-(* Lemma gen_segblocks_in_valid : forall p id sbmap, *)
-(*   In id (map segid (list_of_segments p)) -> *)
-(*   sbmap = gen_segblocks p -> *)
-(*   segblock_is_valid init_block (length (list_of_segments p)) (sbmap id). *)
-(* Proof. *)
-(*   clear. *)
-(*   intros p id sbmap H H0. *)
-(*   assert (length (list_of_segments p) = length (map segid (list_of_segments p))). *)
-(*   { rewrite list_length_map. auto. } *)
-(*   rewrite H1. unfold gen_segblocks in H0. *)
-(*   eapply acc_segblocks_in_valid; eauto. *)
-(* Qed. *)
+Lemma gen_segblocks_in_valid : forall p id sbmap,
+  In id (map segid (list_of_segments p)) ->
+  sbmap = gen_segblocks p ->
+  segblock_is_valid init_block (length (list_of_segments p)) (sbmap id).
+Proof.
+  clear.
+  intros p id sbmap H H0.
+  assert (length (list_of_segments p) = length (map segid (list_of_segments p))).
+  { rewrite list_length_map. auto. }
+  rewrite H1. unfold gen_segblocks in H0.
+  eapply acc_segblocks_in_valid; eauto.
+Qed.
 
-(* Lemma acc_segblocks_range: forall ids b initb initmap s, *)
-(*   b = (acc_segblocks initb ids initmap s) -> *)
-(*   b = (initmap s) \/ segblock_is_valid initb (length ids) b. *)
-(* Proof. *)
-(*   induction ids; simpl; intros. *)
-(*   - auto. *)
-(*   - destruct ident_eq; subst. *)
-(*     + right. red. split. apply Ple_refl. *)
-(*       simpl. rewrite psucc_advance_Nsucc_eq. *)
-(*       apply Pos.le_lt_trans with (pos_advance_N initb (Datatypes.length ids)). *)
-(*       apply pos_advance_N_ple. apply Plt_succ. *)
-(*     + exploit (IHids (acc_segblocks (Pos.succ initb) ids initmap s)); eauto. *)
-(*       intros [ACC | VALID]. *)
-(*       auto. right. unfold segblock_is_valid in *. destruct VALID. *)
-(*       split. apply Ple_trans with (Pos.succ initb); auto. apply Ple_succ. *)
-(*       simpl. auto. *)
-(* Qed. *)
+Lemma acc_segblocks_range: forall ids b initb initmap s,
+  b = (acc_segblocks initb ids initmap s) ->
+  b = (initmap s) \/ segblock_is_valid initb (length ids) b.
+Proof.
+  induction ids; simpl; intros.
+  - auto.
+  - destruct ident_eq; subst.
+    + right. red. split. apply Ple_refl.
+      simpl. rewrite psucc_advance_Nsucc_eq.
+      apply Pos.le_lt_trans with (pos_advance_N initb (Datatypes.length ids)).
+      apply pos_advance_N_ple. apply Plt_succ.
+    + exploit (IHids (acc_segblocks (Pos.succ initb) ids initmap s)); eauto.
+      intros [ACC | VALID].
+      auto. right. unfold segblock_is_valid in *. destruct VALID.
+      split. apply Ple_trans with (Pos.succ initb); auto. apply Ple_succ.
+      simpl. auto.
+Qed.
 
-(* Lemma acc_segblocks_absurd : forall ids b initb initmap s, *)
-(*   (forall s, Plt (initmap s) b) -> Plt b initb -> *)
-(*   b = (acc_segblocks initb ids initmap s) -> False. *)
-(* Proof. *)
-(*   intros. apply acc_segblocks_range in H1. destruct H1. *)
-(*   - subst. specialize (H s). specialize (Plt_strict (initmap s)). *)
-(*     congruence. *)
-(*   - red in H1. destruct H1. generalize (Plt_le_absurd b initb); eauto. *)
-(* Qed. *)
+Lemma acc_segblocks_absurd : forall ids b initb initmap s,
+  (forall s, Plt (initmap s) b) -> Plt b initb ->
+  b = (acc_segblocks initb ids initmap s) -> False.
+Proof.
+  intros. apply acc_segblocks_range in H1. destruct H1.
+  - subst. specialize (H s). specialize (Plt_strict (initmap s)).
+    congruence.
+  - red in H1. destruct H1. generalize (Plt_le_absurd b initb); eauto.
+Qed.
 
-(* Lemma acc_segblocks_injective : forall ids init_block0 initmap sbmap, *)
-(*     (forall s, Plt (initmap s) init_block0) -> *)
-(*     sbmap = acc_segblocks init_block0 ids initmap -> *)
-(*     injective_on_valid_segs init_block0 (length ids) sbmap. *)
-(* Proof. *)
-(*   induction ids; intros. *)
-(*   - simpl in *. subst. red. *)
-(*     intros s1 s2 EQ VALID. *)
-(*     red in VALID. simpl in VALID. *)
-(*     destruct VALID as [VALID1 VALID2]. exfalso. *)
-(*     generalize (Plt_le_absurd (initmap s1) init_block0); eauto. *)
-(*   - simpl in H0. subst. red. intros. repeat destruct ident_eq. *)
-(*     + subst. auto. *)
-(*     + red in H1. destruct H1. *)
-(*       exfalso. eapply (acc_segblocks_absurd ids init_block0 (Psucc init_block0)); eauto. *)
-(*       apply Pos.lt_succ_r. apply Ple_refl. *)
-(*     + red in H1. destruct H1. *)
-(*       exfalso. eapply (acc_segblocks_absurd ids init_block0 (Psucc init_block0)); eauto. *)
-(*       apply Pos.lt_succ_r. apply Ple_refl. *)
-(*     + set (sbmap := acc_segblocks (Pos.succ init_block0) ids initmap) in *. *)
-(*       generalize (IHids (Pos.succ init_block0) initmap sbmap). intros. *)
-(*       exploit H2; eauto. intros. apply Plt_trans_succ. auto. *)
-(*       set (b1 := sbmap s1) in *. *)
-(*       assert (b1 = sbmap s2) by auto. subst sbmap. *)
-(*       apply acc_segblocks_range in H3. destruct H3; auto. *)
-(*       red in H1. destruct H1. specialize (H s2). rewrite <- H3 in H. *)
-(*       exfalso. generalize (Plt_le_absurd b1 init_block0); eauto. *)
-(* Qed. *)
+Lemma acc_segblocks_injective : forall ids init_block0 initmap sbmap,
+    (forall s, Plt (initmap s) init_block0) ->
+    sbmap = acc_segblocks init_block0 ids initmap ->
+    injective_on_valid_segs init_block0 (length ids) sbmap.
+Proof.
+  induction ids; intros.
+  - simpl in *. subst. red.
+    intros s1 s2 EQ VALID.
+    red in VALID. simpl in VALID.
+    destruct VALID as [VALID1 VALID2]. exfalso.
+    generalize (Plt_le_absurd (initmap s1) init_block0); eauto.
+  - simpl in H0. subst. red. intros. repeat destruct ident_eq.
+    + subst. auto.
+    + red in H1. destruct H1.
+      exfalso. eapply (acc_segblocks_absurd ids init_block0 (Psucc init_block0)); eauto.
+      apply Pos.lt_succ_r. apply Ple_refl.
+    + red in H1. destruct H1.
+      exfalso. eapply (acc_segblocks_absurd ids init_block0 (Psucc init_block0)); eauto.
+      apply Pos.lt_succ_r. apply Ple_refl.
+    + set (sbmap := acc_segblocks (Pos.succ init_block0) ids initmap) in *.
+      generalize (IHids (Pos.succ init_block0) initmap sbmap). intros.
+      exploit H2; eauto. intros. apply Plt_trans_succ. auto.
+      set (b1 := sbmap s1) in *.
+      assert (b1 = sbmap s2) by auto. subst sbmap.
+      apply acc_segblocks_range in H3. destruct H3; auto.
+      red in H1. destruct H1. specialize (H s2). rewrite <- H3 in H.
+      exfalso. generalize (Plt_le_absurd b1 init_block0); eauto.
+Qed.
 
-(* Lemma gen_segblocks_injective : forall p, *)
-(*     injective_on_valid_segs init_block (length (list_of_segments p)) (gen_segblocks p). *)
-(* Proof. *)
-(*   intros p. set (sbmap := gen_segblocks p) in *. *)
-(*   unfold gen_segblocks in *. *)
-(*   assert (length (list_of_segments p) = length (map segid (list_of_segments p))). *)
-(*   symmetry. apply list_length_map. rewrite H. *)
-(*   eapply acc_segblocks_injective; eauto. *)
-(*   instantiate (1:=(fun _ : segid_type => undef_seg_block)). intros. simpl. *)
-(*   apply Plt_succ. auto. *)
-(* Qed. *)
+Lemma gen_segblocks_injective : forall p,
+    injective_on_valid_segs init_block (length (list_of_segments p)) (gen_segblocks p).
+Proof.
+  intros p. set (sbmap := gen_segblocks p) in *.
+  unfold gen_segblocks in *.
+  assert (length (list_of_segments p) = length (map segid (list_of_segments p))).
+  symmetry. apply list_length_map. rewrite H.
+  eapply acc_segblocks_injective; eauto.
+  instantiate (1:=(fun _ : segid_type => undef_seg_block)). intros. simpl.
+  apply Plt_succ. auto.
+Qed.
 
 
 Definition empty_genv (p:program): genv :=
@@ -1077,32 +1078,8 @@ Definition lblmap_to_symbmap (smap: segid_type -> block) (lmap:LABEL_MAP_TYPE) :
     | Some (sid,ofs) => Some (smap sid, ofs)
     end.
 
-Definition segmap := 
-  fun sid => if eq_block sid code_segid then 
-            code_block 
-          else 
-            if eq_block sid data_segid then
-              data_block
-            else
-              undef_seg_block.
-
-Lemma segmap_injective: 
-  injective_on_valid_segs code_block 2 segmap.
-Proof.
-  clear.
-  unfold segmap. red. intros.
-  repeat destruct eq_block; subst; auto.
-  unfold data_block, code_block in H. admit.
-  unfold code_block, undef_seg_block in H. admit.
-  unfold data_block, code_block in H. admit.
-  unfold data_block, undef_seg_block in H. admit.
-  unfold undef_seg_block, code_block in H. admit.
-  unfold data_block, undef_seg_block in H. admit.
-  unfold segblock_is_valid in H0. inv H0. admit.
-Admitted.
-
 Definition globalenv (p: program) : genv :=
-  let smap := segmap in
+  let smap := gen_segblocks p in
   let symbmap := gidmap_to_symbmap smap (glob_map p) in
   let lblmap := lblmap_to_symbmap smap (lbl_map p) in
   let imap := gen_instrs_map smap p in
@@ -1242,7 +1219,7 @@ Definition init_mem (p: program) :=
   match alloc_globals m2 (prog_defs p) with
   | None => None
   | Some m3 =>
-    store_globals ge segmap m3 (prog_defs p)
+    store_globals ge (gen_segblocks p) m3 (prog_defs p)
   end.
 
 
